SkLean/Candidates2.lean
@@ -1,41 +1,89 @@
 import SkLean.Ast2
-import SkLean.Typing2
 import SkLean.Sn2
 
-def is_candidate_for (e : Expr) (t : Expr) : Prop := valid_judgment e t ∧ e.valid_universes
+inductive is_candidate_for_n : ℕ → Expr → Expr → Prop
+  | stuck : (¬(∃ e', is_eval_once e e'))
+    → valid_judgment e t
+    → is_candidate_for_n 0 e t
+  | step  : is_eval_once e e'
+    → is_candidate_for_n n e' t'
+    → e.valid_universes
+    → is_candidate_for_n n.succ e t
 
 namespace valid_judgment
 
-lemma imp_is_candidate_for : valid_judgment e t → is_candidate_for e t := by
-  intro h_t
-  unfold is_candidate_for
-  induction h_t
-  constructor
-  apply valid_judgment.k
+lemma imp_valid_universes : valid_judgment e t → e.valid_universes := by
+  intro h
+  induction h
   apply Expr.valid_universes.k
-  constructor
-  apply valid_judgment.s
   apply Expr.valid_universes.s
-  constructor
-  apply valid_judgment.m
   apply Expr.valid_universes.m
-  case call lhs rhs h_u h_t_lhs h_t_rhs ih₁ ih₂ =>
-    simp_all
-    constructor
-    apply valid_judgment.call
+  apply Expr.valid_universes.call
+  case call.a lhs rhs h_u h_t_lhs h_t_rhs h_u_lhs h_u_rhs =>
     exact h_u
-    simp_all
-    simp_all
-    apply Expr.valid_universes.call
+  case call.a lhs rhs h_u h_t_lhs h_t_rhs h_u_lhs h_u_rhs =>
+    exact h_u_lhs
+  case call.a lhs rhs h_u h_t_lhs h_t_rhs h_u_lhs h_u_rhs =>
+    exact h_u_rhs
+
+end valid_judgment
+
+namespace is_candidate_for_n
+
+lemma imp_valid_universes : is_candidate_for_n n e t → e.valid_universes := by
+  intro h
+  induction h
+  case stuck e' t' h_stuck h_t =>
+    apply h_t.imp_valid_universes
+  case step e e' t' t'' h_eval h_candidate h_u _ =>
     exact h_u
-    simp_all
-    simp_all
+
+end is_candidate_for_n
+
+namespace valid_judgment
+
+lemma imp_well_typed_lhs_rhs : valid_judgment SKM[(lhs rhs)] SKM[((M SKM[(lhs rhs)].max_universe.succ) (lhs rhs))] → valid_judgment lhs SKM[((M lhs.max_universe.succ) lhs)] ∧ valid_judgment rhs SKM[((M rhs.max_universe.succ) rhs)] := by
+  intro h_t
+  cases h_t
+  simp_all
+
+lemma imp_is_candidate_for : valid_judgment e t → ∃ n, is_candidate_for_n n e t := by
+  intro h_t
+  induction h_t
+  use 0
+  apply is_candidate_for_n.stuck
+  intro h
+  obtain ⟨e', h⟩ := h
+  cases h
+  apply valid_judgment.k
+  use 0
+  apply is_candidate_for_n.stuck
+  intro h
+  obtain ⟨e', h⟩ := h
+  cases h
+  apply valid_judgment.s
+  use 0
+  apply is_candidate_for_n.stuck
+  intro h
+  obtain ⟨e', h⟩ := h
+  cases h
+  apply valid_judgment.m
+  case call lhs rhs h_u h_t_lhs h_t_rhs h_candidate_lhs h_candidate_rhs =>
+    if h_eval : ∃ e', is_eval_once SKM[(lhs rhs)] e' then
+      obtain ⟨e', h_eval⟩ := h_eval
+      apply @is_candidate_for_n.step _ e'
+      exact h_eval
+      
+      sorry
+    else
+      apply is_candidate_for.stuck
+      exact h_eval
 
 end valid_judgment
 
 namespace is_candidate_for
 
-lemma imp_sn : is_candidate_for e t → sn e := fun ⟨h_t_lhs, h_t_rhs⟩ => by
+lemma imp_sn : is_candidate_for_n e t → sn e := fun ⟨_, h_t_lhs, h_t_rhs⟩ => by
   induction h_t_lhs
   apply sn.k
   apply sn.s
@@ -49,8 +97,11 @@ lemma imp_sn : is_candidate_for e t → sn e := fun ⟨h_t_lhs, h_t_rhs⟩ => by
     match h : SKM[(lhs rhs)] with
       | SKM[(((K n) x) y)] =>
         simp_all
+        apply sn.hard
+        intro e' h
+        cases h
         cases h_t_lhs
-        case intro h_left _ =>
+        case a.k.intro a b c h_left e =>
           cases h_left
       | SKM[((((S n) x) y) z)] =>
         simp_all
@@ -59,14 +110,24 @@ lemma imp_sn : is_candidate_for e t → sn e := fun ⟨h_t_lhs, h_t_rhs⟩ => by
           cases h_left
       | SKM[((M n) e)] =>
         simp_all
-        cases h_t_lhs
-        case intro h_left _ =>
-          cases h_left
+        apply sn.hard
+        intro e' h_eval
+        induction e
+        cases h_eval
+        apply sn.m
+        cases h_eval
+        apply sn.k
+        cases h_eval
+        apply sn.s
+        case a.call a b c d e f g =>
+          induction ih
+          sorry
       | SKM[(lhs rhs)] =>
         simp_all
         cases h_t_lhs
         case intro h_left _ =>
           cases h_left
+          
       | SKM[S rhs] =>
         simp_all
       | SKM[K rhs] =>
@@ -89,5 +150,8 @@ theorem imp_sn : valid_judgment e t → sn e := by
   apply is_candidate_for.imp_sn
   apply imp_is_candidate_for
   exact h_t
+
+lemma imp_sn_weak : valid_judgment e t → beta_eq t t' → sn e := by
+  sorry
 
 end valid_judgment
