SkLean/Checker.lean
@@ -1,0 +1,50 @@
+import SkLean.Ast2
+import SkLean.Typing2
+import SkLean.Candidates2
+
+inductive maybe_typed : Expr → Prop
+  | none : maybe_typed e
+  | some : (∃ t, valid_judgment e t) → maybe_typed e
+
+def type_of (e : Expr) : maybe_typed e :=
+  match e with
+    | SKM[(M n)] => maybe_typed.some ⟨SKM[(M n.succ)], ⟨
+      valid_judgment.m n,
+      by
+        apply beta_eq.symm
+        apply beta_eq.eval
+        apply is_eval_once.m_final
+        apply valid_judgment.m
+      ⟩⟩
+    | SKM[(S n)] => maybe_typed.some ⟨SKM[(S n.succ)], ⟨
+      valid_judgment.s n,
+      by
+        apply beta_eq.symm
+        apply beta_eq.eval
+        apply is_eval_once.m_final
+        apply valid_judgment.s
+      ⟩⟩
+    | SKM[(K n)] => maybe_typed.some ⟨SKM[(K n.succ)], ⟨
+      valid_judgment.k n,
+      by
+        apply beta_eq.symm
+        apply beta_eq.eval
+        apply is_eval_once.m_final
+        apply valid_judgment.k
+      ⟩⟩
+    | SKM[(lhs rhs)] =>
+      if h : lhs.max_universe > rhs.max_universe then
+        match type_of lhs with
+          | .none => .none
+          | .some ⟨t_lhs, h_t_lhs⟩ =>
+            match type_of rhs with
+              | .none => .none
+              | .some ⟨t_rhs, h_t_rhs⟩ =>
+                have h : valid_judgment SKM[(lhs rhs)] SKM[(((M lhs.max_universe.succ) lhs) ((M rhs.max_universe.succ) rhs))] := by
+                  apply valid_judgment.call
+                  exact h
+                  
+                  sorry
+            sorry
+      else
+        maybe_typed.none
