SkLean/Sn2.lean
@@ -1,5 +1,4 @@
 import SkLean.Ast2
-import SkLean.Typing2
 import Mathlib.Tactic
 
 inductive sn : Expr → Prop
@@ -33,14 +32,11 @@ lemma call_k : sn SKM[(((K n) x) y)] ↔ sn x := by
   intro e' h_eval
   cases h_eval
   exact h_sn
-  case mpr.a.left lhs' h =>
-    cases h
-    case left lhs' h =>
-      cases h
 
 lemma call_s : sn SKM[((((S n) x) y) z)] ↔ sn SKM[((x z) (y z))] := by
   constructor
   intro h_sn
+
   match h_sn with
     | .hard h_step =>
       exact h_step SKM[((x z) (y z))] (by apply is_eval_once.s)
@@ -49,18 +45,6 @@ lemma call_s : sn SKM[((((S n) x) y) z)] ↔ sn SKM[((x z) (y z))] := by
   intro e' h_eval
   cases h_eval
   exact h_sn
-  case mpr.a.left lhs' h =>
-    cases h
-    case left lhs' h =>
-      cases h
-      case left lhs' h =>
-        cases h
-
-lemma call_m : sn SKM[((M e.max_universe.succ) e)] → valid_judgment e t → sn t := by
-  intro h_sn h_t
-  match h_sn with
-    | .hard h_step =>
-      exact h_step t (by apply is_eval_once.m_final; exact h_t)
 
 lemma preserved : sn e → is_eval_once e e' → sn e' := by
   intro h_sn h_eval
@@ -89,8 +73,6 @@ lemma imp_n_steps_eval_normal (e : Expr) : valid_judgment e t → sn e → ∃ n
     use SKM[S n]
     apply is_normal_n.s_stuck
   case call lhs rhs h₁ h₂ =>
-    cases h_t
-    case call h₁' h₂' h₃' =>
-      cases h₁'
+    sorry
 
 end sn
