SkLean/Typing2.lean
@@ -2,18 +2,29 @@ import SkLean.Ast2
 
 namespace valid_judgment
 
-lemma preserved : ∀ e e' t, valid_judgment e t → is_eval_once e e' → valid_judgment e' t := by
-  intro e e' t h_t h_eval
-  induction h_t
-  cases h_eval
-  cases h_eval
-  cases h_eval
-  case call lhs rhs h_u h_t_lhs h_t_rhs ih₁ ih₂ =>
+theorem preservation_easy : valid_judgment e t → is_eval_once e e' → ∃ t', valid_judgment e' t' := by
+  intro h_t h_eval
+  induction h_eval
+  cases h_t
+  case k.call_k _ _ t_x h_t_x =>
+    use t_x
+  case s x y z n =>
+    cases h_t
+    case call_s t_call h_t_call h_u =>
+      use t_call
+  cases h_t
+  cases h_t
+  cases h_t
+  cases h_t
+  case left lhs lhs' rhs h_eval ih =>
+    cases h_t
     cases h_eval
-    cases h_t_lhs
-    cases h_t_lhs
-    cases h_t_lhs
-    cases h_t_lhs
-    cases h_t_lhs
+    case call_k.left x t_x n h_t_ lhs' h_eval =>
+      cases h_eval
+    cases h_eval
+    case call_s.left x t_x n h_t_ lhs' h_eval =>
+      cases h_eval
+      case left x y z h_eval =>
+        cases h_eval
 
 end valid_judgment
